examples/Rewrite.v
@@ -22,14 +22,271 @@ Inductive Fooish {T} : Foo T -> Foo T -> Prop :=
 | AS : forall x, Fooish (A x) (A x)
 | BS : forall x y, Fooish (B x) (B y).
 
-(*
+(* 
 Instance GenSizedSuchThat_foo :
   GenSizedSuchThat _ (fun '(x,y) => Fooish x y) :=
   { arbitrarySizeST := fun n => returnGen (Some (A,A)) }.
 
 Sample (@arbitraryST _ (fun '(x,y) => Fooish x y) _).
  *)
-QuickChickDebug Debug On.
+QuickChickDebug Debug On. Check @forAll.
+
+Derive Generator for (fun ft => Fooish ft ft'). Print Coq.Init.Nat.one.
+Derive Checker for (Fooish a b).
+Derive Enumerator for (fun ft => Fooish ft ft').
+(**
+
+Definition a := (@QuickChick.Checker.forAllMaybe _ _ _ _ (@QuickChick.DependentClasses.arbitraryST _ (fun 'e' => @bigstep' e e') _)
+   (fun 'e' =>
+    @Quickchick.Checker.forAllMaybe _ _ _ _ (@QuickChick.DependentClasses.arbitraryST _ (fun 'e => @typing' Gamma e tau) _)
+      (fun 'e =>
+       @Quickchick.Checker.forAll _ _ _ _ (@Quickchick.Classes.arbitrary (@type) _)
+         (fun 'tau =>
+          @Quickchick.Checker.forAll _ _ _ _ (@Quickchick.Classes.arbitrary (@list (@type)) _)
+            (fun 'Gamma =>
+             match @Quickchick.Decidability.decOpt (@typing' Gamma e' tau) _ Quickchick.Decidability.checkable_size_limit with
+             | @Some _ (@true) =>
+                 @Quickchick.Checker.checker _ _ (@Coq.Init.Datatypes.Some Coq.Init.Datatypes.bool Coq.Init.Datatypes.true)
+             | @Some _ (@false) =>
+                 @Quickchick.Checker.checker _ _ (@Coq.Init.Datatypes.Some Coq.Init.Datatypes.bool Coq.Init.Datatypes.false)
+             | @None => @Quickchick.Checker.checker _ _ Coq.Init.Datatypes.tt
+             end))))).*)
+
+Theorem qaegweg : @Fooish nat (A 0) (A 0).
+Proof. 
+
+  Fixpoint blah n := match n with | 0 => 0 | S n => S (blah n) end
+
+  with blur n := match n with | 0 => 0 | S n => S (S (blur n)) end.
+  
+Abort.
+
+Inductive type := N | Arrow (i o : type).
+
+Inductive term :=
+| Const (n : nat)
+| App (f x : term)
+| Abs (ty : type) (e : term)
+| Id (x : nat)
+.
+
+Print blur.
+
+Inductive bind : list type -> nat -> type -> Prop :=
+| BindNow   : forall tau env, bind (tau :: env) O tau
+| BindLater : forall tau tau' x env,
+    bind env x tau -> bind (tau' :: env) (S x) tau.
+
+  Inductive typing (G : list type) : term -> type -> Prop :=
+  | TId :
+      forall x t,
+        bind G x t ->
+        typing G (Id x) t
+  | TConst :
+      forall n,
+        typing G (Const n) N
+  | TAbs :
+      forall e t1 t2,
+        typing (t1 :: G) e t2 ->
+        typing G (Abs t1 e) (Arrow t1 t2)
+  | TApp :
+      forall e1 e2 t1 t2,
+        typing G e2 t1 ->
+        typing G e1 (Arrow t1 t2) ->
+        typing G (App e1 e2) t2.
+
+
+#[global] Instance Dec_Eqtype (t t' : type) : Dec (t = t').
+Proof. dec_eq. Defined.
+Derive DecOpt for (bind env x t).
+Derive EnumSized for type.
+Derive Enumerator for (fun ty => typing env e ty).
+
+
+
+Definition check_typing := (fix rec init_size size G e tau :=
+   match size with
+   | @Coq.Init.Datatypes.O =>
+       @QuickChick.Decidability.checker_backtrack
+         (@Coq.Init.Datatypes.cons _
+            (fun '_ =>
+             match tau with
+             | t =>
+                 match e with
+                 | @Id x =>
+                     @QuickChick.Decidability.andBind
+                       (@QuickChick.Decidability.decOpt (@bind G x t) _ QuickChick.Decidability.checkable_size_limit)
+                       (@Coq.Init.Datatypes.Some Coq.Init.Datatypes.bool Coq.Init.Datatypes.true)
+                 | _ => @Coq.Init.Datatypes.None _
+                 end
+             end)
+            (@Coq.Init.Datatypes.cons _
+               (fun '_ =>
+                match tau with
+                | @N =>
+                    match e with
+                    | @Const n => @Coq.Init.Datatypes.Some Coq.Init.Datatypes.bool Coq.Init.Datatypes.true
+                    | _ => @Coq.Init.Datatypes.None _
+                    end
+                | _ => @Coq.Init.Datatypes.None _
+                end) (@Coq.Init.Datatypes.nil _)))
+   | @Coq.Init.Datatypes.S size' =>
+       @QuickChick.Decidability.checker_backtrack
+         (@Coq.Init.Datatypes.cons _
+            (fun '_ =>
+             match tau with
+             | t =>
+                 match e with
+                 | @Id x =>
+                     @QuickChick.Decidability.andBind
+                       (@QuickChick.Decidability.decOpt (@bind G x t) _ QuickChick.Decidability.checkable_size_limit)
+                       (@Coq.Init.Datatypes.Some Coq.Init.Datatypes.bool Coq.Init.Datatypes.true)
+                 | _ => @Coq.Init.Datatypes.None _
+                 end
+             end)
+            (@Coq.Init.Datatypes.cons _
+               (fun '_ =>
+                match tau with
+                | @N =>
+                    match e with
+                    | @Const n => @Coq.Init.Datatypes.Some Coq.Init.Datatypes.bool Coq.Init.Datatypes.true
+                    | _ => @Coq.Init.Datatypes.None _
+                    end
+                | _ => @Coq.Init.Datatypes.None _
+                end)
+               (@Coq.Init.Datatypes.cons _
+                  (fun '_ =>
+                   match tau with
+                   | @Arrow t1' t2 =>
+                       match e with
+                       | @Abs t1 e =>
+                           @QuickChick.Decidability.andBind
+                             (@QuickChick.Decidability.decOpt (@eq (@type) t1 t1') _ QuickChick.Decidability.checkable_size_limit)
+                             (@QuickChick.Decidability.andBind
+                                (rec init_size size' (cons t1 G) e t2)
+                                (@Coq.Init.Datatypes.Some Coq.Init.Datatypes.bool Coq.Init.Datatypes.true))
+                       | _ => @Coq.Init.Datatypes.None _
+                       end
+                   | _ => @Coq.Init.Datatypes.None _
+                   end)
+                  (@Coq.Init.Datatypes.cons _
+                     (fun '_ =>
+                      match tau with
+                      | t2 =>
+                          match e with
+                          | @App e1 e2 =>
+                              @QuickChick.Enumerators.enumeratingOpt _
+                                (@QuickChick.DependentClasses.enumSuchThat _ (fun t1 => @typing G e2 t1) _)
+                                (fun t1 =>
+                                 @QuickChick.Decidability.andBind
+                                   (rec init_size size' G e1 (@Arrow t1 t2))
+                                   (@Coq.Init.Datatypes.Some Coq.Init.Datatypes.bool Coq.Init.Datatypes.true)) init_size
+                          | _ => @Coq.Init.Datatypes.None _
+                          end
+                      end) (@Coq.Init.Datatypes.nil _)))))
+   end).
+
+Check check_typing.
+
+Print check_typing.
+
+Derive Checker for (typing G e ty).
+
+Compute check_typing.
+
+Compute (check_typing 100 100 nil (Const 0) N).
+
+Locate bindOpt.
+
+Definition gen_bind := (let name_Gen :=
+   fix rec init_size size (env : list type) :=
+     match size with
+     | @Coq.Init.Datatypes.O =>
+         @QuickChick.Generators.backtrack _
+           (@Coq.Init.Datatypes.cons _
+              (@Coq.Init.Datatypes.pair _ _ Coq.Init.Nat.one
+                 (@QuickChick.Generators.thunkGen _
+                    (fun '_ =>
+                     match env with
+                     | @cons _ tau env => @QuickChick.Generators.returnGen _ (@Coq.Init.Datatypes.Some _ (@pair _ _ (@O) tau))
+                     | _ => @QuickChick.Generators.returnGen _ (@Coq.Init.Datatypes.None _)
+                     end))) (@Coq.Init.Datatypes.nil _))
+     | @Coq.Init.Datatypes.S size' =>
+         @QuickChick.Generators.backtrack _
+           (@Coq.Init.Datatypes.cons _
+              (@Coq.Init.Datatypes.pair _ _ Coq.Init.Nat.one
+                 (@QuickChick.Generators.thunkGen _
+                    (fun '_ =>
+                     match env with
+                     | @cons _ tau env => @QuickChick.Generators.returnGen _ (@Coq.Init.Datatypes.Some _ (@pair _ _ (@O) tau))
+                     | _ => @QuickChick.Generators.returnGen _ (@Coq.Init.Datatypes.None _)
+                     end)))
+              (@Coq.Init.Datatypes.cons _
+                 (@Coq.Init.Datatypes.pair _ _ size
+                    (@QuickChick.Generators.thunkGen _
+                       (fun '_ =>
+                        match env with
+                        | @cons _ tau' env =>
+                            @QuickChick.Producer.bindOpt _ _ _ _ (@rec init_size size' env)
+                              (fun '(@Coq.Init.Datatypes.pair _ _ x tau) =>
+                               @QuickChick.Generators.returnGen _ (@Coq.Init.Datatypes.Some _ (@pair _ _ (@S x) tau)))
+                        | _ => @QuickChick.Generators.returnGen _ (@Coq.Init.Datatypes.None _)
+                        end))) (@Coq.Init.Datatypes.nil _)))
+     end in
+                        fun size => @name_Gen size size).
+
+Definition gen_bind' := (let bind_iooGen :=
+   fix rec
+     (init_size : Coq.Init.Datatypes.nat) (size : Coq.Init.Datatypes.nat)
+     (env : @list (@type)) :=
+     match size with
+     | @Coq.Init.Datatypes.O =>
+         @QuickChick.Generators.backtrack _
+           (@Coq.Init.Datatypes.cons _
+              (@Coq.Init.Datatypes.pair _ _ Coq.Init.Nat.one
+                 (@QuickChick.Generators.thunkGen _
+                    (fun '_ =>
+                     match env with
+                     | @cons _ tau env =>
+                         @QuickChick.Generators.returnGen _
+                           (@Coq.Init.Datatypes.Some _ (@pair _ _ (@O) tau))
+                     | _ =>
+                         @QuickChick.Generators.returnGen _ (@Coq.Init.Datatypes.None _)
+                     end))) (@Coq.Init.Datatypes.nil _))
+     | @Coq.Init.Datatypes.S size' =>
+         @QuickChick.Generators.backtrack _
+           (@Coq.Init.Datatypes.cons _
+              (@Coq.Init.Datatypes.pair _ _ Coq.Init.Nat.one
+                 (@QuickChick.Generators.thunkGen _
+                    (fun '_ =>
+                     match env with
+                     | @cons _ tau env =>
+                         @QuickChick.Generators.returnGen _
+                           (@Coq.Init.Datatypes.Some _ (@pair _ _ (@O) tau))
+                     | _ =>
+                         @QuickChick.Generators.returnGen _ (@Coq.Init.Datatypes.None _)
+                     end)))
+              (@Coq.Init.Datatypes.cons _
+                 (@Coq.Init.Datatypes.pair _ _ size
+                    (@QuickChick.Generators.thunkGen _
+                       (fun '_ =>
+                        match env with
+                        | @cons _ tau' env =>
+                            @QuickChick.Producer.bindOpt _ _ _ _
+                              (@rec init_size size' env)
+                              (fun '(@Coq.Init.Datatypes.pair _ _ x tau) =>
+                               @QuickChick.Generators.returnGen _
+                                 (@Coq.Init.Datatypes.Some _ (@pair _ _ (@S x) tau)))
+                        | _ =>
+                            @QuickChick.Generators.returnGen _
+                              (@Coq.Init.Datatypes.None _)
+                        end))) (@Coq.Init.Datatypes.nil _)))
+     end in
+ fun size : Coq.Init.Datatypes.nat => @bind_iooGen size size).
+
+Check gen_bind'. Locate nat.
+
+QuickChickDebug Debug Off.
 Derive Testing for (fun '(x,y,z,w) => Fooish x y z). 
 Derive Testing for (Fooish x y). 
 Derive Testing for (fun x => Fooish x y). 
